Port refinement rules from Iris examples.

test.v
@@ -1,61 +1,454 @@
 From mathcomp Require Import ssreflect.
-From iris.algebra Require Import gmap auth gset numbers.
+From iris.algebra Require Import excl auth frac agree gmap list.
+From iris.proofmode Require Import tactics.
+From iris.program_logic Require Export language ectx_language ectxi_language.
+From iris.program_logic Require Import lifting.
+From iris.algebra Require Import gmap auth gset numbers excl agree ofe.
 From iris.heap_lang Require Import notation proofmode metatheory.
+From iris.heap_lang Require Import primitive_laws.
 From iris.base_logic.lib Require Import invariants.
+Import uPred.
 
-Class symbolG Σ := { symbol_inG :> inG Σ (authR max_natUR) }.
-Definition symbolΣ : gFunctors := #[GFunctor (authR max_natUR)].
+Definition specN := nroot .@ "spec".
 
-Section Symbol.
+(** The CMRA for the heap of the specification. *)
+Definition tpoolUR : ucmraT := gmapUR nat (exclR exprO).
+Definition cfgUR := prodUR tpoolUR (gen_heapUR loc (optionO valO)).
 
-Context `{!symbolG Σ, heapG Σ}.
+Fixpoint to_tpool_go (i : nat) (tp : list expr) : tpoolUR :=
+  match tp with
+  | [] => ∅
+  | e :: tp => <[i:=Excl e]>(to_tpool_go (S i) tp)
+  end.
+Definition to_tpool : list expr → tpoolUR := to_tpool_go 0.
 
-Implicit Types (γ : gname) (l : loc) (n : nat).
+(** The CMRA for the thread pool. *)
+Class cfgSG Σ := CFGSG { cfg_inG :> inG Σ (authR cfgUR); cfg_name : gname }.
 
-Definition counterN := nroot .@ "counter".
+Section definitionsS.
+  Context `{cfgSG Σ, invG Σ}.
 
-Definition symbol γ v :=
-  (∃ n : nat, ⌜v = #n⌝ ∗ own γ (◯ (MaxNat (S n))))%I.
-Definition counter γ v :=
-  (∃ l : loc, ⌜v = #l⌝ ∗
-     inv (counterN .@ l)
-       (∃ n : nat, (l ↦ #n) ∗ own γ (● (MaxNat n))))%I.
+  Definition heapS_mapsto (l : loc) (q : Qp) (v: valO) : iProp Σ :=
+    own cfg_name (◯ (ε, {[ l := (q, to_agree (Some v : leibnizO (option val))) ]})).
 
-Definition symbol_init : val := λ: <>, ref #0.
+  Definition tpool_mapsto (j : nat) (e: expr) : iProp Σ :=
+    own cfg_name (◯ ({[ j := Excl e ]}, ∅)).
 
-Lemma wp_symbol_init :
-  ⊢ WP symbol_init #() {{v, ∃ γ, counter γ v}}.
-Proof.
-iIntros; iApply wp_fupd.
-rewrite /symbol_init; wp_alloc l as "Hl".
-iPoseProof (own_alloc (● (MaxNat 0))) as "H".
-  by apply/auth_auth_valid.
-iMod "H"; iDestruct "H" as (γ) "Hγ".
-pose (has n := own γ (● (MaxNat n))).
-iMod (inv_alloc (counterN.@l) _ (∃ n : nat, (l ↦ #n) ∗ has n) with "[Hl Hγ]").
-  iNext; iExists 0; iFrame.
-iModIntro; iExists γ. iExists l. iFrame. eauto.
-Qed.
+  Definition spec_inv (ρ : cfg heap_lang) : iProp Σ :=
+    (∃ tp (σ : state),
+      own cfg_name (● (to_tpool tp, to_gen_heap (heap σ)))
+      ∗ ⌜rtc erased_step ρ (tp,σ)⌝)%I.
+  Definition spec_ctx : iProp Σ :=
+    (∃ ρ, inv specN (spec_inv ρ))%I.
 
-Definition symbol_new : val := λ: "l", FAA "l" #1.
+  Global Instance heapS_mapsto_timeless l q v : Timeless (heapS_mapsto l q v).
+  Proof. apply _. Qed.
+  Global Instance spec_ctx_persistent : Persistent spec_ctx.
+  Proof. apply _. Qed.
+End definitionsS.
+Typeclasses Opaque heapS_mapsto tpool_mapsto.
 
-Lemma wp_symbol_new γ v :
-  counter γ v -∗
-  WP symbol_new v {{w, symbol γ w}}.
-Proof.
-iDestruct 1 as (l) "[-> #?]".
-rewrite /symbol_new; wp_pures.
-iInv (counterN.@l) as (n) "[> Hl > Hn]"; wp_faa.
-pose m := MaxNat (S n).
-iPoseProof (own_update _ _ (● m ⋅ ◯ m) with "Hn") as "> Hn".
-  apply auth_update_alloc.
-  apply max_nat_local_update.
-  rewrite /=; lia.
-rewrite own_op; iDestruct "Hn" as "[Hn1 Hn2]"; iModIntro.
-iSplit.
-- iNext. iExists (S n).
-  rewrite Nat2Z.inj_succ -Z.add_1_r; by iFrame.
-- by iExists n; iSplit.
-Qed.
+Notation "l ↦ₛ{ q } v" := (heapS_mapsto l q v)
+  (at level 20, q at level 50, format "l  ↦ₛ{ q }  v") : bi_scope.
+Notation "l ↦ₛ v" := (heapS_mapsto l 1 v) (at level 20) : bi_scope.
+Notation "j ⤇ e" := (tpool_mapsto j e) (at level 20) : bi_scope.
 
-End Symbol.
+Ltac iAsimpl :=
+  repeat match goal with
+  | |- context [ (_ ⤇ ?e)%I ] => progress (
+    let e' := fresh in evar (e':expr);
+    assert (e = e') as ->; [simpl; unfold e'; reflexivity|];
+    unfold e'; clear e')
+  | |- context [ WP ?e @ _ {{ _ }}%I ] => progress (
+    let e' := fresh in evar (e':expr);
+    assert (e = e') as ->; [simpl; unfold e'; reflexivity|];
+    unfold e'; clear e')
+  end.
+
+Section conversions.
+  Context `{cfgSG Σ}.
+
+  (** Conversion to tpools and back *)
+  Lemma to_tpool_valid es : ✓ to_tpool es.
+  Proof.
+    rewrite /to_tpool. move: 0.
+    induction es as [|e es]=> n //. by apply insert_valid.
+  Qed.
+
+  Lemma tpool_lookup tp j : to_tpool tp !! j = Excl <$> tp !! j.
+  Proof.
+    cut (∀ i, to_tpool_go i tp !! (i + j) = Excl <$> tp !! j).
+    { intros help. apply (help 0). }
+    revert j. induction tp as [|e tp IH]=> //= -[|j] i /=.
+    - by rewrite Nat.add_0_r lookup_insert.
+    - by rewrite -Nat.add_succ_comm lookup_insert_ne; last lia.
+  Qed.
+  Lemma tpool_lookup_Some tp j e : to_tpool tp !! j = Excl' e → tp !! j = Some e.
+  Proof. rewrite tpool_lookup fmap_Some. naive_solver. Qed.
+  Hint Resolve tpool_lookup_Some : core.
+
+  Lemma to_tpool_insert tp j e :
+    j < length tp →
+    to_tpool (<[j:=e]> tp) = <[j:=Excl e]> (to_tpool tp).
+  Proof.
+    intros. apply: map_eq=> i. destruct (decide (i = j)) as [->|].
+    - by rewrite tpool_lookup lookup_insert list_lookup_insert.
+    - rewrite tpool_lookup lookup_insert_ne // list_lookup_insert_ne //.
+      by rewrite tpool_lookup.
+  Qed.
+  Lemma to_tpool_insert' tp j e :
+    is_Some (to_tpool tp !! j) →
+    to_tpool (<[j:=e]> tp) = <[j:=Excl e]> (to_tpool tp).
+  Proof.
+    rewrite tpool_lookup fmap_is_Some lookup_lt_is_Some. apply to_tpool_insert.
+  Qed.
+
+  Lemma to_tpool_snoc tp e :
+    to_tpool (tp ++ [e]) = <[length tp:=Excl e]>(to_tpool tp).
+  Proof.
+    intros. apply: map_eq=> i.
+    destruct (lt_eq_lt_dec i (length tp)) as [[?| ->]|?].
+    - rewrite lookup_insert_ne; last lia. by rewrite !tpool_lookup lookup_app_l.
+    - by rewrite lookup_insert tpool_lookup lookup_app_r // Nat.sub_diag.
+    - rewrite lookup_insert_ne; last lia.
+      rewrite !tpool_lookup ?lookup_ge_None_2 ?app_length //=;
+         change (ofe_car exprO) with expr; lia.
+  Qed.
+
+  Lemma tpool_singleton_included tp j e :
+    {[j := Excl e]} ≼ to_tpool tp → tp !! j = Some e.
+  Proof.
+    move=> /singleton_included_l [ex [/leibniz_equiv_iff]].
+    rewrite tpool_lookup fmap_Some=> [[e' [-> ->]] /Excl_included ?]. by f_equal.
+  Qed.
+  Lemma tpool_singleton_included' tp j e :
+    {[j := Excl e]} ≼ to_tpool tp → to_tpool tp !! j = Excl' e.
+  Proof. rewrite tpool_lookup. by move=> /tpool_singleton_included=> ->. Qed.
+
+End conversions.
+
+Section cfg.
+  Context `{heapG Σ, cfgSG Σ}.
+  Implicit Types P Q : iProp Σ.
+  Implicit Types Φ : val → iProp Σ.
+  Implicit Types σ : state.
+  Implicit Types e : expr.
+  Implicit Types l : loc.
+  Implicit Types v : val.
+  Implicit Types a b : Z.
+
+  Local Hint Resolve tpool_lookup : core.
+  Local Hint Resolve tpool_lookup_Some : core.
+  Local Hint Resolve to_tpool_insert : core.
+  Local Hint Resolve to_tpool_insert' : core.
+  Local Hint Resolve tpool_singleton_included : core.
+
+  Lemma mapstoS_agree l q1 q2 v1 v2 : l ↦ₛ{q1} v1 -∗ l ↦ₛ{q2} v2 -∗ ⌜v1 = v2⌝.
+  Proof.
+    apply wand_intro_r.
+    rewrite /heapS_mapsto -own_op -auth_frag_op own_valid discrete_valid.
+    f_equiv=> -[_] /=. rewrite singleton_op singleton_valid -pair_op.
+    by intros [_ ?%agree_op_invL']; congruence.
+  Qed.
+  Lemma mapstoS_combine l q1 q2 v1 v2 :
+    l ↦ₛ{q1} v1 -∗ l ↦ₛ{q2} v2 -∗ l ↦ₛ{q1 + q2} v1 ∗ ⌜v1 = v2⌝.
+  Proof.
+    iIntros "Hl1 Hl2". iDestruct (mapstoS_agree with "Hl1 Hl2") as %->.
+    rewrite /heapS_mapsto. iCombine "Hl1 Hl2" as "Hl". eauto with iFrame.
+  Qed.
+  Lemma mapstoS_valid l q v : l ↦ₛ{q} v -∗ ✓ q.
+  Proof.
+    rewrite /heapS_mapsto own_valid !discrete_valid -auth_frag_valid.
+    by apply pure_mono=> -[_] /singleton_valid [??].
+  Qed.
+  Lemma mapstoS_valid_2 l q1 q2 v1 v2 : l ↦ₛ{q1} v1 -∗ l ↦ₛ{q2} v2 -∗ ✓ (q1 + q2)%Qp.
+  Proof.
+    iIntros "H1 H2". iDestruct (mapstoS_combine with "H1 H2") as "[? ->]".
+    by iApply (mapstoS_valid l _ v2).
+  Qed.
+
+  Lemma step_insert K tp j e σ κ e' σ' efs :
+    tp !! j = Some (fill K e) → head_step e σ κ e' σ' efs →
+    erased_step (tp, σ) (<[j:=fill K e']> tp ++ efs, σ').
+  Proof.
+    intros. rewrite -(take_drop_middle tp j (fill K e)) //.
+    rewrite insert_app_r_alt take_length_le ?Nat.sub_diag /=;
+      eauto using lookup_lt_Some, Nat.lt_le_incl.
+    rewrite -(assoc_L (++)) /=. eexists.
+    eapply step_atomic; eauto. by apply: Ectx_step'.
+  Qed.
+
+  Lemma step_insert_no_fork K tp j e σ κ e' σ' :
+    tp !! j = Some (fill K e) → head_step e σ κ e' σ' [] →
+    erased_step (tp, σ) (<[j:=fill K e']> tp, σ').
+  Proof. rewrite -(right_id_L [] (++) (<[_:=_]>_)). by apply step_insert. Qed.
+
+  Lemma nsteps_inv_r {A} n (R : A → A → Prop) x y :
+    relations.nsteps R (S n) x y → ∃ z, relations.nsteps R n x z ∧ R z y.
+  Proof.
+    revert x y; induction n; intros x y.
+    - inversion 1; subst.
+      match goal with H : relations.nsteps _ 0 _ _ |- _ => inversion H end; subst.
+      eexists; repeat econstructor; eauto.
+    - inversion 1; subst.
+      edestruct IHn as [z [? ?]]; eauto.
+      exists z; split; eauto using relations.nsteps_l.
+  Qed.
+
+  Lemma step_pure' E j K e e' (P : Prop) n :
+    P →
+    PureExec P n e e' →
+    nclose specN ⊆ E →
+    spec_ctx ∗ j ⤇ fill K e ={E}=∗ j ⤇ fill K e'.
+  Proof.
+    iIntros (HP Hex ?) "[#Hinv Hj]". iDestruct "Hinv" as (ρ) "Hspec".
+    rewrite /spec_ctx /tpool_mapsto.
+    iInv specN as (tp σ) ">[Hown Hrtc]" "Hclose".
+    iDestruct "Hrtc" as %Hrtc.
+    iDestruct (own_valid_2 with "Hown Hj")
+      as %[[Htpj%tpool_singleton_included' _]%prod_included ?]%auth_both_valid.
+    iMod (own_update_2 with "Hown Hj") as "[Hown Hj]".
+    { by eapply auth_update, prod_local_update_1,
+        singleton_local_update, (exclusive_local_update _ (Excl (fill K e'))). }
+    iFrame "Hj". iApply "Hclose". iNext. iExists (<[j:=fill K e']> tp), σ.
+    rewrite to_tpool_insert'; last eauto.
+    iFrame. iPureIntro.
+    apply rtc_nsteps in Hrtc; destruct Hrtc as [m Hrtc].
+    specialize (Hex HP). apply (nsteps_rtc (m + n)).
+    eapply nsteps_trans; eauto.
+    revert e e' Htpj Hex.
+    induction n => e e' Htpj Hex.
+    - inversion Hex; subst.
+      rewrite list_insert_id; eauto. econstructor.
+    - apply nsteps_inv_r in Hex.
+      destruct Hex as [z [Hex1 Hex2]].
+      specialize (IHn _ _ Htpj Hex1).
+      eapply nsteps_r; eauto.
+      replace (<[j:=fill K e']> tp) with
+          (<[j:=fill K e']> (<[j:=fill K z]> tp)); last first.
+      { clear. revert tp; induction j; intros tp.
+        - destruct tp; trivial.
+        - destruct tp; simpl; auto. by rewrite IHj. }
+      destruct Hex2 as [Hexs Hexd].
+      specialize (Hexs σ). destruct Hexs as [e'' [σ' [efs Hexs]]].
+      specialize (Hexd σ [] e'' σ' efs Hexs); destruct Hexd as [? [? [? ?]]];
+        subst.
+      inversion Hexs; simpl in *; subst.
+      rewrite -!fill_app.
+      eapply step_insert_no_fork; eauto.
+      { apply list_lookup_insert. apply lookup_lt_is_Some; eauto. }
+  Qed.
+
+
+  Lemma do_step_pure E j K e e' `{!PureExec True 1 e e'}:
+    nclose specN ⊆ E →
+    spec_ctx ∗ j ⤇ fill K e ={E}=∗ j ⤇ fill K e'.
+  Proof. by eapply step_pure'; last eauto. Qed.
+
+  Lemma step_alloc E j K v:
+    nclose specN ⊆ E →
+    spec_ctx ∗ j ⤇ fill K (Alloc v) ={E}=∗ ∃ l, j ⤇ fill K #l ∗ l ↦ₛ v.
+  Proof.
+    iIntros (?) "[#Hinv Hj]". iDestruct "Hinv" as (ρ) "Hinv".
+    rewrite /spec_ctx /tpool_mapsto.
+    iInv specN as (tp σ) ">[Hown %]" "Hclose".
+    destruct (exist_fresh (dom (gset loc) (heap σ))) as [l Hl%not_elem_of_dom].
+    iDestruct (own_valid_2 with "Hown Hj")
+      as %[[?%tpool_singleton_included' _]%prod_included ?]%auth_both_valid.
+    iMod (own_update_2 with "Hown Hj") as "[Hown Hj]".
+    { by eapply auth_update, prod_local_update_1,
+        singleton_local_update, (exclusive_local_update _ (Excl (fill K #l))). }
+    iMod (own_update with "Hown") as "[Hown Hl]".
+    { eapply auth_update_alloc, prod_local_update_2,
+        (alloc_singleton_local_update _ l (1%Qp,to_agree (Some v : leibnizO _)));
+        last done.
+      by apply lookup_to_gen_heap_None. }
+    iExists l. rewrite /heapS_mapsto. iFrame "Hj Hl". iApply "Hclose". iNext.
+    iExists (<[j:=fill K #l]> tp), (state_init_heap l 1 v σ).
+    rewrite {1}state_init_heap_singleton /=.
+    rewrite to_gen_heap_insert to_tpool_insert'; last eauto. iFrame. iPureIntro.
+    eapply rtc_r, step_insert_no_fork; eauto.
+    eapply AllocNS; first lia.
+    move=> i ??; rewrite (_ : i = 0) /= ?loc_add_0 //.
+    lia.
+  Qed.
+
+  Lemma step_load E j K l q v:
+    nclose specN ⊆ E →
+    spec_ctx ∗ j ⤇ fill K (Load #l) ∗ l ↦ₛ{q} v
+    ={E}=∗ j ⤇ fill K (of_val v) ∗ l ↦ₛ{q} v.
+  Proof.
+    iIntros (?) "(#Hinv & Hj & Hl)". iDestruct "Hinv" as (ρ) "Hinv".
+    rewrite /spec_ctx /tpool_mapsto /heapS_mapsto.
+    iInv specN as (tp σ) ">[Hown %]" "Hclose".
+    iDestruct (own_valid_2 with "Hown Hj")
+      as %[[?%tpool_singleton_included' _]%prod_included ?]%auth_both_valid.
+    iDestruct (own_valid_2 with "Hown Hl")
+      as %[[? ?%gen_heap_singleton_included]%prod_included ?]%auth_both_valid.
+    iMod (own_update_2 with "Hown Hj") as "[Hown Hj]".
+    { by eapply auth_update, prod_local_update_1, singleton_local_update,
+        (exclusive_local_update _ (Excl (fill K (of_val v)))). }
+    iFrame "Hj Hl". iApply "Hclose". iNext.
+    iExists (<[j:=fill K (of_val v)]> tp), σ.
+    rewrite to_tpool_insert'; last eauto. iFrame. iPureIntro.
+    eapply rtc_r, step_insert_no_fork; eauto. econstructor; eauto.
+  Qed.
+
+  Lemma step_store E j K l v' v:
+    nclose specN ⊆ E →
+    spec_ctx ∗ j ⤇ fill K (Store #l v) ∗ l ↦ₛ v'
+    ={E}=∗ j ⤇ fill K #() ∗ l ↦ₛ v.
+  Proof.
+    iIntros (?) "(#Hinv & Hj & Hl)". iDestruct "Hinv" as (ρ) "Hinv".
+    rewrite /spec_ctx /tpool_mapsto /heapS_mapsto.
+    iInv specN as (tp σ) ">[Hown %]" "Hclose".
+    iDestruct (own_valid_2 with "Hown Hj")
+      as %[[?%tpool_singleton_included' _]%prod_included _]%auth_both_valid.
+    iDestruct (own_valid_2 with "Hown Hl")
+      as %[[_ Hl%gen_heap_singleton_included]%prod_included _]%auth_both_valid.
+    iMod (own_update_2 with "Hown Hj") as "[Hown Hj]".
+    { by eapply auth_update, prod_local_update_1, singleton_local_update,
+        (exclusive_local_update _ (Excl (fill K #()))). }
+    iMod (own_update_2 with "Hown Hl") as "[Hown Hl]".
+    { eapply auth_update, prod_local_update_2, singleton_local_update,
+        (exclusive_local_update _ (1%Qp, to_agree (Some v : leibnizO _))); last done.
+      by rewrite /to_gen_heap lookup_fmap Hl. }
+    iFrame "Hj Hl". iApply "Hclose". iNext.
+    iExists (<[j:=fill K #()]> tp), (state_upd_heap <[l:=Some v]> σ).
+    rewrite to_gen_heap_insert to_tpool_insert'; last eauto. iFrame. iPureIntro.
+    eapply rtc_r, step_insert_no_fork; eauto.
+    econstructor; eauto.
+  Qed.
+
+  Lemma step_cas_fail E j K l q v' v1 v2:
+    nclose specN ⊆ E → v' ≠ v1 →
+    vals_compare_safe v' v1 ->
+    spec_ctx ∗ j ⤇ fill K (CmpXchg #l v1 v2) ∗ l ↦ₛ{q} v'
+    ={E}=∗ j ⤇ fill K (v', #false)%V ∗ l ↦ₛ{q} v'.
+  Proof.
+    iIntros (???) "(#Hinv & Hj & Hl)". iDestruct "Hinv" as (ρ) "Hinv".
+    rewrite /spec_ctx /tpool_mapsto /heapS_mapsto.
+    iInv specN as (tp σ) ">[Hown %]" "Hclose".
+    iDestruct (own_valid_2 with "Hown Hj")
+      as %[[?%tpool_singleton_included' _]%prod_included ?]%auth_both_valid.
+    iDestruct (own_valid_2 with "Hown Hl")
+      as %[[_ ?%gen_heap_singleton_included]%prod_included _]%auth_both_valid.
+    iMod (own_update_2 with "Hown Hj") as "[Hown Hj]".
+    { by eapply auth_update, prod_local_update_1, singleton_local_update,
+        (exclusive_local_update _ (Excl (fill K (v', #false)%V))). }
+    iFrame "Hj Hl". iApply "Hclose". iNext.
+    iExists (<[j:=fill K (v', #false)%V]> tp), σ.
+    rewrite to_tpool_insert'; last eauto. iFrame. iPureIntro.
+    eapply rtc_r, step_insert_no_fork; eauto.
+    change σ with (if false then state_upd_heap <[l:=Some v2]> σ else σ) at 3.
+    econstructor; eauto.
+    by apply/eq_sym/bool_decide_eq_false.
+  Qed.
+
+  Lemma step_cas_suc E j K l v1 v1' v2:
+    nclose specN ⊆ E → v1 = v1' →
+    vals_compare_safe v1 v1' →
+    spec_ctx ∗ j ⤇ fill K (CmpXchg #l v1 v2) ∗ l ↦ₛ v1'
+    ={E}=∗ j ⤇ fill K (v1', #true)%V ∗ l ↦ₛ v2.
+  Proof.
+    iIntros (???) "(#Hinv & Hj & Hl)"; subst. iDestruct "Hinv" as (ρ) "Hinv".
+    rewrite /spec_ctx /tpool_mapsto /heapS_mapsto.
+    iInv specN as (tp σ) ">[Hown %]" "Hclose".
+    iDestruct (own_valid_2 with "Hown Hj")
+      as %[[?%tpool_singleton_included' _]%prod_included _]%auth_both_valid.
+    iDestruct (own_valid_2 with "Hown Hl")
+      as %[[_ Hl%gen_heap_singleton_included]%prod_included _]%auth_both_valid.
+    iMod (own_update_2 with "Hown Hj") as "[Hown Hj]".
+    { by eapply auth_update, prod_local_update_1, singleton_local_update,
+        (exclusive_local_update _ (Excl (fill K (v1', #true)%V))). }
+    iMod (own_update_2 with "Hown Hl") as "[Hown Hl]".
+    { eapply auth_update, prod_local_update_2, singleton_local_update,
+        (exclusive_local_update _ (1%Qp, to_agree (Some v2 : leibnizO _))); last done.
+      by rewrite /to_gen_heap lookup_fmap Hl. }
+    iFrame "Hj Hl". iApply "Hclose". iNext.
+    iExists (<[j:=fill K (v1', #true)%V]> tp), (state_upd_heap <[l:=Some v2]> σ).
+    rewrite -[state_upd_heap <[l:=Some v2]> σ]/(if true then state_upd_heap <[l:=Some v2]> σ else σ).
+    rewrite to_gen_heap_insert to_tpool_insert'; last eauto. iFrame. iPureIntro.
+    eapply rtc_r, step_insert_no_fork; eauto.
+    econstructor; eauto.
+    by apply/eq_sym/bool_decide_eq_true.
+  Qed.
+
+  Lemma step_rec E j K f x v1 v2 `{!AsRecV v1 f x erec}:
+    nclose specN ⊆ E →
+    spec_ctx ∗ j ⤇ fill K (App v1 v2)
+    ={E}=∗ j ⤇ fill K (subst' x v2 (subst' f v1 erec)).
+  Proof. move=> ?; by apply: do_step_pure. Qed.
+
+  Lemma step_lam E j K x e1 v2 :
+    nclose specN ⊆ E →
+    spec_ctx ∗ j ⤇ fill K (App (λ: x, e1)%V v2)
+    ={E}=∗ j ⤇ fill K (subst' x v2 e1).
+  Proof.
+    move=> ?. iIntros "H".
+    iPoseProof (step_rec with "H") as "H"; eauto.
+  Qed.
+
+  Lemma step_fst E j K v1 v2 :
+    nclose specN ⊆ E →
+    spec_ctx ∗ j ⤇ fill K (Fst (v1, v2)%V) ={E}=∗ j ⤇ fill K v1.
+  Proof. by intros; apply: do_step_pure. Qed.
+
+  Lemma step_snd E j K v1 v2 :
+    nclose specN ⊆ E →
+    spec_ctx ∗ j ⤇ fill K (Snd (v1, v2)%V) ={E}=∗ j ⤇ fill K v2.
+  Proof. by intros; apply: do_step_pure. Qed.
+
+  Lemma step_case_inl E j K v0 e1 e2 :
+    nclose specN ⊆ E →
+    spec_ctx ∗ j ⤇ fill K (Case (InjLV v0)%V e1 e2)
+      ={E}=∗ j ⤇ fill K (e1 v0).
+  Proof. by intros; apply: do_step_pure. Qed.
+
+  Lemma step_case_inr E j K v0 e1 e2 :
+    nclose specN ⊆ E →
+    spec_ctx ∗ j ⤇ fill K (Case (InjRV v0)%V e1 e2)
+      ={E}=∗ j ⤇ fill K (e2 v0).
+  Proof. by intros; apply: do_step_pure. Qed.
+
+  Lemma step_if_false E j K e1 e2 :
+    nclose specN ⊆ E →
+    spec_ctx ∗ j ⤇ fill K (If #false e1 e2) ={E}=∗ j ⤇ fill K e2.
+  Proof. by intros; apply: do_step_pure. Qed.
+
+  Lemma step_if_true E j K e1 e2 :
+    nclose specN ⊆ E →
+    spec_ctx ∗ j ⤇ fill K (If #true e1 e2) ={E}=∗ j ⤇ fill K e1.
+  Proof. by intros; apply: do_step_pure. Qed.
+
+  Lemma step_nat_binop E j K op v1 v2 v :
+    nclose specN ⊆ E →
+    bin_op_eval op v1 v2 = Some v →
+    spec_ctx ∗ j ⤇ fill K (BinOp op v1 v2)
+      ={E}=∗ j ⤇ fill K v.
+  Proof. by intros; apply: step_pure'. Qed.
+
+  Lemma step_fork E j K e :
+    nclose specN ⊆ E →
+    spec_ctx ∗ j ⤇ fill K (Fork e) ={E}=∗ ∃ j', j ⤇ fill K #() ∗ j' ⤇ e.
+  Proof.
+    iIntros (?) "[#Hinv Hj]". iDestruct "Hinv" as (ρ) "Hinv".
+    rewrite /spec_ctx /tpool_mapsto.
+    iInv specN as (tp σ) ">[Hown %]" "Hclose".
+    iDestruct (own_valid_2 with "Hown Hj")
+      as %[[?%tpool_singleton_included' _]%prod_included ?]%auth_both_valid.
+    assert (j < length tp) by eauto using lookup_lt_Some.
+    iMod (own_update_2 with "Hown Hj") as "[Hown Hj]".
+    { by eapply auth_update, prod_local_update_1,
+        singleton_local_update, (exclusive_local_update _ (Excl (fill K #()))). }
+    iMod (own_update with "Hown") as "[Hown Hfork]".
+    { eapply auth_update_alloc, prod_local_update_1,
+        (alloc_singleton_local_update _ (length tp) (Excl e)); last done.
+      rewrite lookup_insert_ne ?tpool_lookup; last lia.
+      by rewrite lookup_ge_None_2. }
+    iExists (length tp). iFrame "Hj Hfork". iApply "Hclose". iNext.
+    iExists (<[j:=fill K #()]> tp ++ [e]), σ.
+    rewrite to_tpool_snoc insert_length to_tpool_insert //. iFrame. iPureIntro.
+    eapply rtc_r, step_insert; eauto. econstructor; eauto.
+  Qed.
+End cfg.
